@prefix : <https://core-eq.nbnl.info/vocab/> .
@prefix cim: <https://cim.ucaiug.io/ns#> .
# @prefix dct: <http://purl.org/dc/terms/> .
# @prefix dcterms: <http://purl.org/dc/terms/> .
@prefix nbnl-term: <https://nbnl.info/thesaurus/ebs/> .
# @prefix owl: <http://www.w3.org/2002/07/owl#> .
@prefix rdf: <http://www.w3.org/1999/02/22-rdf-syntax-ns#> .
@prefix rdfs: <http://www.w3.org/2000/01/rdf-schema#> .
# @prefix sh: <http://www.w3.org/ns/shacl#> .
@prefix skos: <http://www.w3.org/2004/02/skos/core#> .
# @prefix skosxl: <http://www.w3.org/2008/05/skos-xl#> .
@prefix xsd: <http://www.w3.org/2001/XMLSchema#> .

# :0001 a rdfs:Class ;
#     rdfs:label "MarketEvaluationPoint" ;
#     rdfs:subClassOf cim:MarketEvaluationPoint ;
#     skos:definition "..." .

# OR:
cim:MarketEvaluationPoint a rdfs:Class ;
    rdfs:label "MarketEvaluationPoint" ;
    skos:definition "The identification of an entity where energy products are measured"@en ,
                    "De identificatie van een entiteit waar energieproducten gemeten worden"@nl ;
    rdfs:isDefinedBy cim: .

:0001 a rdf:Property ;
    rdfs:label "sbiCodes" ;
    skos:exactMatch nbnl-term:sbiCodes ;
    # skosxl:altLabel [
    #     skos:scopeNote "Python" ;
    #     skosxl:literalForm "sbi_codes"
    # ] , [
    #     skos:scopeNote "Java" ;
    #     skosxl:literalForm "sbiCodes"

    # ] ;
    skos:definition "Standaard BedrijfsIndeling code. Used by the Dutch Chamber of Commerce to classify activities performed by an organisation."@en ;
    rdfs:domain :0001 ;
    # OR:
    # rdfs:domain cim:MarketEvaluationPoint ;
    rdfs:range xsd:string .

    
# OR:
# :0002 a rdf:Property ;
#     rdfs:label "sbiCodes" ;
#     skos:exactMatch nbnl-term:sbiCodes ;
#     skosxl:altLabel [
#         skos:scopeNote "Python" ;
#         skosxl:literalForm "sbi_codes"
#     ] , [
#         skos:scopeNote "Java" ;
#         skosxl:literalForm "sbiCodes"

#     ] ;
#     skos:definition "Standaard BedrijfsIndeling code. Used by the Dutch Chamber of Commerce to classify activities performed by an organisation."@en ;
#     rdfs:domain :0001 ;
#     # OR:
#     # rdfs:domain cim:MarketEvaluationPoint ;
#     rdfs:range xsd:string .